open import lib
open import VarInterface

module Tm(vi : VI) where

open VI vi

data Tm : Set where
  var : (x : V) â†’ Tm
  _Â·_ : (t : Tm) â†’ (t' : Tm) â†’ Tm
  Æ› : (x : V) â†’ (t : Tm) â†’ Tm

infixl 10 _Â·_ 

-- is the given variable free in the given term
freeIn : V â†’ Tm â†’ Set
freeIn x (var y) = x â‰ƒ y â‰¡ tt
freeIn x (t Â· t') = (freeIn x t) âˆ¨ (freeIn x t')
freeIn x (Æ› y t) = x â‰ƒ y â‰¡ ff âˆ§ freeIn x t

-- is the given variable free in the given term
boundIn : V â†’ Tm â†’ Set
boundIn x (var y) = âŠ¥
boundIn x (t Â· t') = (boundIn x t) âˆ¨ (boundIn x t')
boundIn x (Æ› y t) = x â‰ƒ y â‰¡ tt âˆ¨ boundIn x t

bv-apart : Tm â†’ Tm â†’ Set
bv-apart t2 t1 = âˆ€ (x : V) â†’ freeIn x t2 â†’ Â¬ boundIn x t1

bv-apart-app : âˆ€{t2 t1a t1b : Tm} â†’
                bv-apart t2 (t1a Â· t1b) â†’
                bv-apart t2 t1a âˆ§ bv-apart t2 t1b
bv-apart-app{t2}{t1a}{t1b} a = (Î» x u b â†’ a x u (injâ‚ b)) , Î» x u b â†’ a x u (injâ‚‚ b)

bv-apart-app' : âˆ€{t2 t1a t1b : Tm} â†’
                bv-apart t2 t1a â†’
                bv-apart t2 t1b â†’ 
                bv-apart t2 (t1a Â· t1b)
bv-apart-app'{t2}{t1a}{t1b} a1 a2 x u (injâ‚ b) = a1 x u b
bv-apart-app'{t2}{t1a}{t1b} a1 a2 x u (injâ‚‚ b) = a2 x u b

bv-apart-lam : âˆ€{t2 : Tm}{x : V}{t1 : Tm} â†’
                bv-apart t2 (Æ› x t1) â†’
                Â¬ freeIn x t2 âˆ§ bv-apart t2 t1
bv-apart-lam{t2}{x}{t1} u = (Î» f â†’ u x f (injâ‚ (â‰ƒ-refl {x}))) , Î» y f b â†’ u y f (injâ‚‚ b)

Â¬freeIn-app : âˆ€{x : V}{t t' : Tm} â†’
               Â¬ freeIn x (t Â· t') â†’
               Â¬ (freeIn x t) âˆ§ Â¬ (freeIn x t')
Â¬freeIn-app{x}{t}{t'} nf = (Î» f â†’ nf (injâ‚ f)) , (Î» f â†’ nf (injâ‚‚ f))

Â¬freeIn-lam : âˆ€{x y : V}{t : Tm} â†’
               Â¬ freeIn x (Æ› y t) â†’
               x â‰ƒ y â‰¡ tt âˆ¨ (x â‰ƒ y â‰¡ ff âˆ§ Â¬ freeIn x t)
Â¬freeIn-lam{x}{y}{t} nf with x â‰ƒ y
Â¬freeIn-lam{x}{y}{t} nf | tt = injâ‚ refl
Â¬freeIn-lam{x}{y}{t} nf | ff = injâ‚‚ (refl , (Î» f â†’ nf (refl , f)))

fv : Tm â†’ ğ•ƒ V
fv (var x) = [ x ]
fv (t1 Â· t2) = fv t1 ++ fv t2
fv (Æ› x t) = remove _â‰ƒ_ x (fv t)